coq/theories/assembly/ASMToString.v
@@ -41,44 +41,184 @@ Fixpoint clean (cs: string) (acc: string): string :=
 
 Definition inst2str (i: instr) (str: string): string :=
   match i with
-  | Const r imm => "movq $" ++ N2str (Z.to_N (word.unsigned imm)) (", " ++ reg2str1 r str)
-  | Mov dst src => "movq " ++ reg2str1 src (", " ++ reg2str1 dst str)
-  | ASMSyntax.Add dst src => "addq " ++ reg2str1 src (", " ++ reg2str1 dst str)
-  | Sub dst src => "subq " ++ reg2str1 src (", " ++ reg2str1 dst str)
-  | Div r => "divq " ++ reg2str1 r str
+  | Const r imm => 
+    let prefix := "movq $" in
+    let imm_unsigned := word.unsigned imm in
+    let imm_n := Z.to_N imm_unsigned in
+    let comma_str := ", " in
+    let reg_str := reg2str1 r str in
+    let comma_reg := comma_str ++ reg_str in
+    let imm_str := N2str imm_n comma_reg in
+    prefix ++ imm_str
+  | Mov dst src => 
+    let prefix := "movq " in
+    let src_str := reg2str1 src in
+    let comma_str := ", " in
+    let dst_str := reg2str1 dst str in
+    let comma_dst := comma_str ++ dst_str in
+    let src_comma_dst := src_str comma_dst in
+    prefix ++ src_comma_dst
+  | ASMSyntax.Add dst src => 
+    let prefix := "addq " in
+    let src_str := reg2str1 src in
+    let comma_str := ", " in
+    let dst_str := reg2str1 dst str in
+    let comma_dst := comma_str ++ dst_str in
+    let src_comma_dst := src_str comma_dst in
+    prefix ++ src_comma_dst
+  | Sub dst src => 
+    let prefix := "subq " in
+    let src_str := reg2str1 src in
+    let comma_str := ", " in
+    let dst_str := reg2str1 dst str in
+    let comma_dst := comma_str ++ dst_str in
+    let src_comma_dst := src_str comma_dst in
+    prefix ++ src_comma_dst
+  | Div r => 
+    let prefix := "divq " in
+    let r_str := reg2str1 r str in
+    prefix ++ r_str
   | Jump cond n =>
     match cond with
-    | Always => "jmp " ++ lab n str
+    | Always => 
+      let prefix := "jmp " in
+      let lab_str := lab n str in
+      prefix ++ lab_str
     | Equal r1 r2 =>
-      "cmpq " ++ reg2str1 r2 (", " ++ reg2str1 r1 (" ; je " ++ lab n str))
+      let cmpq_prefix := "cmpq " in
+      let r2_str := reg2str1 r2 in
+      let comma_str := ", " in
+      let je_prefix := " ; je " in
+      let lab_str := lab n str in
+      let je_lab := je_prefix ++ lab_str in
+      let r1_str := reg2str1 r1 je_lab in
+      let comma_r1 := comma_str ++ r1_str in
+      let r2_comma_r1 := r2_str comma_r1 in
+      cmpq_prefix ++ r2_comma_r1
     | Less r1 r2 =>
-      "cmpq " ++ reg2str1 r2 (", " ++ reg2str1 r1 (" ; jb " ++ lab n str))
+      let cmpq_prefix := "cmpq " in
+      let r2_str := reg2str1 r2 in
+      let comma_str := ", " in
+      let jb_prefix := " ; jb " in
+      let lab_str := lab n str in
+      let jb_lab := jb_prefix ++ lab_str in
+      let r1_str := reg2str1 r1 jb_lab in
+      let comma_r1 := comma_str ++ r1_str in
+      let r2_comma_r1 := r2_str comma_r1 in
+      cmpq_prefix ++ r2_comma_r1
     end
-  | Call n => "call " ++ lab n str
-  | Ret => "ret" ++ str
-  | Pop r => "popq " ++ reg2str1 r str
-  | Push r => "pushq " ++ reg2str1 r str
-  | Load_RSP r n => "movq " ++ num2str (8 * n) ("(%rsp), " ++ reg2str1 r str)
-  | Store_RSP r n => "movq " ++ (reg2str1 r (", " ++ num2str (8 * n) ("(%rsp), " ++ str)))
-  | Add_RSP n => "addq $" ++ num2str (8 * n) (", %rsp" ++ str)
-  | Sub_RSP n => "subq $" ++ num2str (8 * n) (", %rsp" ++ str)
+  | Call n => 
+    let prefix := "call " in
+    let lab_str := lab n str in
+    prefix ++ lab_str
+  | Ret => 
+    let prefix := "ret" in
+    prefix ++ str
+  | Pop r => 
+    let prefix := "popq " in
+    let r_str := reg2str1 r str in
+    prefix ++ r_str
+  | Push r => 
+    let prefix := "pushq " in
+    let r_str := reg2str1 r str in
+    prefix ++ r_str
+  | Load_RSP r n => 
+    let prefix := "movq " in
+    let mult_const := 8 in
+    let offset := mult_const * n in
+    let rsp_prefix := "(%rsp), " in
+    let r_str := reg2str1 r str in
+    let rsp_r := rsp_prefix ++ r_str in
+    let offset_str := num2str offset rsp_r in
+    prefix ++ offset_str
+  | Store_RSP r n => 
+    let prefix := "movq " in
+    let comma_str := ", " in
+    let mult_const := 8 in
+    let offset := mult_const * n in
+    let rsp_suffix := "(%rsp), " in
+    let rsp_suffix_str := rsp_suffix ++ str in
+    let offset_str := num2str offset rsp_suffix_str in
+    let comma_offset := comma_str ++ offset_str in
+    let r_str := reg2str1 r comma_offset in
+    prefix ++ r_str
+  | Add_RSP n => 
+    let prefix := "addq $" in
+    let mult_const := 8 in
+    let offset := mult_const * n in
+    let rsp_suffix := ", %rsp" in
+    let rsp_suffix_str := rsp_suffix ++ str in
+    let offset_str := num2str offset rsp_suffix_str in
+    prefix ++ offset_str
+  | Sub_RSP n => 
+    let prefix := "subq $" in
+    let mult_const := 8 in
+    let offset := mult_const * n in
+    let rsp_suffix := ", %rsp" in
+    let rsp_suffix_str := rsp_suffix ++ str in
+    let offset_str := num2str offset rsp_suffix_str in
+    prefix ++ offset_str
   | Store src a w =>
-      "movq " ++ reg2str1 src (", " ++ N2str (Z.to_N (word.unsigned w)) ("(" ++ reg2str1 a (")" ++ str)))
+    let prefix := "movq " in
+    let src_str := reg2str1 src in
+    let comma_str := ", " in
+    let w_unsigned := word.unsigned w in
+    let w_n := Z.to_N w_unsigned in
+    let paren_open := "(" in
+    let paren_close := ")" in
+    let paren_close_str := paren_close ++ str in
+    let a_str := reg2str1 a paren_close_str in
+    let paren_a := paren_open ++ a_str in
+    let w_str := N2str w_n paren_a in
+    let comma_w := comma_str ++ w_str in
+    let src_comma_w := src_str comma_w in
+    prefix ++ src_comma_w
   | Load dst a w =>
-      "movq " ++ N2str (Z.to_N (word.unsigned w)) ("(" ++ reg2str1 a ("), " ++ reg2str1 dst str))
-  | GetChar => "movq stdin(%rip), %rdi ; call _IO_getc@PLT" ++ str
-  | PutChar => "movq stdout(%rip), %rsi ; call _IO_putc@PLT" ++ str
-  | Exit => "call exit@PLT" ++ str
-  | Comment c => "
-  
-  	/* " ++ clean c (" */" ++ str)
+    let prefix := "movq " in
+    let w_unsigned := word.unsigned w in
+    let w_n := Z.to_N w_unsigned in
+    let paren_open := "(" in
+    let paren_close := "), " in
+    let dst_str := reg2str1 dst str in
+    let paren_close_dst := paren_close ++ dst_str in
+    let a_str := reg2str1 a paren_close_dst in
+    let paren_a := paren_open ++ a_str in
+    let w_str := N2str w_n paren_a in
+    prefix ++ w_str
+  | GetChar => 
+    let prefix := "movq stdin(%rip), %rdi ; call _IO_getc@PLT" in
+    prefix ++ str
+  | PutChar => 
+    let prefix := "movq stdout(%rip), %rsi ; call _IO_putc@PLT" in
+    prefix ++ str
+  | Exit => 
+    let prefix := "call exit@PLT" in
+    prefix ++ str
+  | Comment c => 
+    let newline := "
+    
+    	/* " in
+    let suffix := " */" in
+    let suffix_str := suffix ++ str in
+    let clean_c := clean c suffix_str in
+    newline ++ clean_c
   end.
 
 Fixpoint instrs2str (n: nat) (is: asm): string :=
   match is with
   | [] => EmptyString
   | i :: is =>
-    lab n (String ":" (String "009" (inst2str i (String "010" (instrs2str (n+1) is)))))
+    let colon := ":"%char in
+    let tab_char := "009"%char in
+    let newline_char := "010"%char in
+    let next_n := n + 1 in
+    let rest_str := instrs2str next_n is in
+    let newline_rest := String newline_char rest_str in
+    let inst_str := inst2str i newline_rest in
+    let tab_inst := String tab_char inst_str in
+    let colon_tab_inst := String colon tab_inst in
+    let result := lab n colon_tab_inst in
+    result
   end.
 
 Fixpoint concat_strings (ss: list string): string :=
