coq/theories/derivations/ParserDerivations.v
@@ -1,0 +1,177 @@
+From impboot Require Import utils.Core.
+From impboot Require Import utils.AppList.
+Require Import impboot.assembly.ASMSyntax.
+Require Import impboot.assembly.ASMToString.
+Require Import impboot.imperative.ImpSyntax.
+Require Import impboot.utils.AppList.
+Require Import impboot.parsing.Parser.
+Require Import impboot.imp2asm.ImpToASMCodegen.
+From impboot Require Import automation.Ltac2Utils.
+From impboot Require Import commons.PrintingUtils.
+From impboot Require Import functional.FunValues.
+From impboot Require Import functional.FunSemantics.
+Require Import impboot.automation.RelCompiler.
+Require Import impboot.automation.ltac2.UnfoldFix.
+Require Import impboot.automation.AutomationLemmas.
+Require Import coqutil.Word.Interface.
+Require Import ZArith.
+From Stdlib Require Import FunInd.
+From Stdlib Require Import derive.Derive.
+From Stdlib Require Import Lia.
+From Ltac2 Require Import Ltac2.
+
+(* lexing *)
+
+Derive read_num_prog
+  in ltac2:(relcompile_tpe 'read_num_prog 'read_num [])
+  as read_num_prog_proof.
+Proof.
+  time relcompile.
+Qed.
+
+Derive end_line_prog
+  in ltac2:(relcompile_tpe 'end_line_prog 'end_line [])
+  as end_line_prog_proof.
+Proof.
+  time relcompile.
+Qed.
+
+Derive q_from_nat_prog
+  in ltac2:(relcompile_tpe 'q_from_nat_prog 'q_from_nat [])
+  as q_from_nat_prog_proof.
+Proof.
+  time relcompile.
+Qed.
+
+Derive lex_prog
+  in ltac2:(relcompile_tpe 'lex_prog 'lex ['end_line; 'read_num; 'q_from_nat; '@list_length])
+  as lex_prog_proof.
+Proof.
+  time relcompile.
+Qed.
+
+Derive lexer_i_prog
+  in ltac2:(relcompile_tpe 'lexer_i_prog 'lexer_i ['@lex; '@list_length])
+  as lexer_i_prog_proof.
+Proof.
+  time relcompile.
+Qed.
+
+Derive lexer_prog
+  in ltac2:(relcompile_tpe 'lexer_prog 'lexer ['lexer_i])
+  as lexer_prog_proof.
+Proof.
+  time relcompile.
+Qed.
+
+(* parsing *)
+
+Derive quote_prog
+  in ltac2:(relcompile_tpe 'quote_prog 'quote [])
+  as quote_prog_proof.
+Proof.
+  time relcompile.
+Qed.
+
+Derive parse_prog
+  in ltac2:(relcompile_tpe 'parse_prog 'parse [])
+  as parse_prog_proof.
+Proof.
+  time relcompile.
+Qed.
+
+(* converting from v to prog *)
+
+Derive v2list_prog
+  in ltac2:(relcompile_tpe 'v2list_prog 'v2list [])
+  as v2list_prog_proof.
+Proof.
+  time relcompile.
+Qed.
+
+Derive num2exp_prog
+  in ltac2:(relcompile_tpe 'num2exp_prog 'num2exp [])
+  as num2exp_prog_proof.
+Proof.
+  time relcompile.
+Qed.
+
+Derive v2exp_prog
+  in ltac2:(relcompile_tpe 'v2exp_prog 'v2exp [])
+  as v2exp_prog_proof.
+Proof.
+  time relcompile.
+Qed.
+
+Derive vs2exps_prog
+  in ltac2:(relcompile_tpe 'vs2exps_prog 'vs2exps [])
+  as vs2exps_prog_proof.
+Proof.
+  time relcompile.
+Qed.
+
+Derive v2cmp_prog
+  in ltac2:(relcompile_tpe 'v2cmp_prog 'v2cmp [])
+  as v2cmp_prog_proof.
+Proof.
+  time relcompile.
+Qed.
+
+Derive v2test_prog
+  in ltac2:(relcompile_tpe 'v2test_prog 'v2test [])
+  as v2test_prog_proof.
+Proof.
+  time relcompile.
+Qed.
+
+Derive v2cmd_prog
+  in ltac2:(relcompile_tpe 'v2cmd_prog 'v2cmd [])
+  as v2cmd_prog_proof.
+Proof.
+  time relcompile.
+Qed.
+
+Derive vs2args_prog
+  in ltac2:(relcompile_tpe 'vs2args_prog 'vs2args [])
+  as vs2args_prog_proof.
+Proof.
+  time relcompile.
+Qed.
+
+Derive v2func_prog
+  in ltac2:(relcompile_tpe 'v2func_prog 'v2func [])
+  as v2func_prog_proof.
+Proof.
+  time relcompile.
+Qed.
+
+Derive v2funcs_prog
+  in ltac2:(relcompile_tpe 'v2funcs_prog 'v2funcs [])
+  as v2funcs_prog_proof.
+Proof.
+  time relcompile.
+Qed.
+
+Derive vs2prog_prog
+  in ltac2:(relcompile_tpe 'vs2prog_prog 'vs2prog [])
+  as vs2prog_prog_proof.
+Proof.
+  time relcompile.
+Qed.
+
+(* entire parser *)
+
+Derive parser_prog
+  in ltac2:(relcompile_tpe 'parser_prog 'parser [])
+  as parser_prog_proof.
+Proof.
+  time relcompile.
+Qed.
+
+Derive str2imp_prog
+  in ltac2:(relcompile_tpe 'str2imp_prog 'str2imp [])
+  as str2imp_prog_proof.
+Proof.
+  time relcompile.
+Qed.
+
