coq/theories/imp2asm/ImpToASMCodegen.v
@@ -8,7 +8,6 @@ Require Import ZArith.
 Require Import FunInd.
 Require Import Ascii.
 
-
 Require Import impboot.automation.ltac2.UnfoldFix.
 Require Import Ltac2.Ltac2.
 
