coq/theories/parsing/ParserData.v
@@ -1,0 +1,8 @@
+Require Import impboot.utils.Core.
+
+Inductive token :=
+  | OPEN
+  | CLOSE
+  | DOT
+  | NUM (n: N)
+  | QUOTE (s: N).
