coq/theories/parsing/ParserProofs.v
@@ -1,0 +1,72 @@
+Require Import impboot.utils.Core.
+Require Import impboot.parsing.Parser.
+Require Import Patat.Patat.
+
+Ltac cleanup :=
+  repeat match goal with
+  | H: _ /\ _ |- _ => destruct H; clear H
+  | H: (_, _) = (_, _) |- _ => inversion H; clear H; subst
+  end.
+
+Theorem read_num_length: ∀l h xs n ys f acc x,
+  read_num l h f x acc xs = (n, ys) ->
+    List.length ys ≤ List.length xs ∧ (xs ≠ ys -> List.length ys < List.length xs)%nat.
+Proof.
+  induction xs; intros; simpl in *; unfold dlet in *; cleanup; simpl.
+  1: split; eauto; intros; congruence.
+  destruct andb eqn:?; rewrite ?andb_true_iff, ?andb_false_iff, ?N.leb_le, ?N.leb_gt in *; cleanup; simpl in *.
+  1: {
+    pat `read_num _ _ _ _ _ _ = _` at rename pat into Hread_num.
+    pat `forall n ys f acc x, _` at eapply pat in Hread_num.
+    split; [lia|].
+    intros; lia.
+  }
+  split; [lia|].
+  intros; congruence.
+Qed.
+
+Theorem end_line_length: ∀cs,
+  (List.length (end_line cs) <= List.length cs)%nat.
+Proof.
+  induction cs; simpl; unfold dlet in *; [lia|].
+  destruct (_ =? _)%char eqn:?; lia.
+Qed.
+
+Theorem lex_terminates: forall fuel q cs acc,
+  (List.length cs <= fuel)%nat -> lex q cs acc fuel <> None.
+Proof.
+  Opaque Ascii.eqb.
+  induction fuel; intros; simpl; unfold dlet in *.
+  1: inversion H; simpl; destruct cs eqn:?; simpl in *; try congruence.
+  destruct cs eqn:?; try congruence; simpl in *.
+  repeat match goal with
+  | |- (if ?c then _ else _) <> _ => destruct c eqn:?
+  | |- lex _ _ _ _ <> _ =>
+    eapply IHfuel
+  | |- (let (_, _) := if ?c then _ else _ in _) <> _ =>
+    destruct c eqn:?
+  | |- (let (_, _) := read_num _ _ _ _ _ cs in _) <> _ =>
+    destruct read_num eqn:?
+  | H: _ = _ :: ?l |- (let (_, _) := read_num ?a1 ?a2 ?a3 ?a4 ?a5 ?l in _) <> _ =>
+    destruct (read_num a1 a2 a3 a4 a5 l) eqn:?
+  | |- (List.length (end_line _) <= _)%nat =>
+    eapply Nat.le_trans; [eapply end_line_length|]; lia
+  | H: (S _ <= S _)%nat |- _ =>
+    eapply le_S_n in H
+  | H: cs = ?h :: ?t |- (List.length (?h :: ?t) <= _)%nat =>
+    rewrite negb_true_iff, Nat.eqb_neq in *; simpl in *; congruence
+  | H: read_num _ _ _ _ _ ?t = (_, _) |- _ =>
+    eapply read_num_length in H
+  | _ =>
+    progress unfold dlet in *
+  | _ => lia
+  end.
+Qed.
+
+Theorem lexer_terminates: forall (inp: string),
+  lexer_i inp <> None.
+Proof.
+  intros; unfold lexer_i, dlet.
+  eapply lex_terminates.
+  eapply Nat.le_refl.
+Qed.
